Simplify con_two_add, make invariant even more closely match paper

theories/coneris/examples/con_two_add.v
@@ -1,40 +1,10 @@
 From iris.algebra Require Import excl_auth cmra.
-From iris.base_logic.lib Require Import invariants.
+From iris.base_logic.lib Require Import invariants ghost_var.
 From clutch.coneris Require Import coneris par spawn.
 
 Local Open Scope Z.
 
 Set Default Proof Using "Type*".
-
-Section lemmas'.
-  Context `{!inG Σ (excl_authR (boolO))}.
-
-  (* Helpful lemmas *)
-  Lemma ghost_var_alloc' b :
-    ⊢ |==> ∃ γ, own γ (●E b) ∗ own γ (◯E b).
-  Proof.
-    iMod (own_alloc (●E b ⋅ ◯E b)) as (γ) "[??]".
-    - by apply excl_auth_valid.
-    - by eauto with iFrame.
-  Qed.
-
-  Lemma ghost_var_agree' γ b c :
-    own γ (●E b) -∗ own γ (◯E c) -∗ ⌜ b = c ⌝.
-  Proof.
-    iIntros "Hγ● Hγ◯".
-    by iCombine "Hγ● Hγ◯" gives %->%excl_auth_agree_L.
-  Qed.
-
-  Lemma ghost_var_update' γ b' b c :
-    own γ (●E b) -∗ own γ (◯E c) ==∗ own γ (●E b') ∗ own γ (◯E b').
-  Proof.
-    iIntros "Hγ● Hγ◯".
-    iMod (own_update_2 _ _ _ (●E b' ⋅ ◯E b') with "Hγ● Hγ◯") as "[$$]".
-    { by apply excl_auth_update. }
-    done.
-  Qed.
-End lemmas'.
-
 
 (** * This is the con_two_add example in the paper of Coneris*)
 Definition two_add_prog' : expr :=
@@ -47,8 +17,10 @@ Definition two_add_prog' : expr :=
 
 (** * This is the proof sketched for the example con_two_add in the paper of Coneris.
 
-   This is **not** the most idiomatic/direct way to encode this proof, but it is structured to match
-   the simplified layout of the text to avoid pulling in too many high level Iris ideas *)
+   This is **not** the most idiomatic/direct way to encode this proof,
+   but it is structured to match the structure/presentation in the
+   text, where we tried to avoid pulling in too many high level Iris
+   ideas *)
 
 (* Each thread moves through a state machine with 3 states:
 
@@ -63,6 +35,10 @@ Inductive T : Type :=
 | S1 (n : nat) : T
 | S2 (n : nat) : T.
 
+(* Next we define various (pure) predicates that on the states of the
+   threads that capture the informal english descriptions described in
+   the underbraces in the paper *)
+
 Definition no_thread_added t1 t2 :=
   match t1, t2 with
   | S2 _, _ => False
@@ -70,7 +46,7 @@ Definition no_thread_added t1 t2 :=
   | _, _ => True
   end.
 
-Definition one_thread_added t1 t2 n :=
+Definition one_thread_added n t1 t2 :=
   match t1, t2 with
   | S2 _, S2 _ => False
   | S2 n', _ => n = n'
@@ -78,7 +54,7 @@ Definition one_thread_added t1 t2 n :=
   | _, _ => False
   end.
 
-Definition both_threads_added t1 t2 n :=
+Definition both_threads_added n t1 t2 :=
   match t1, t2 with
   | S2 n1, S2 n2 => n = n1 + n2
   | _, _ => False
@@ -89,7 +65,7 @@ Definition no_thread_sampled t1 t2 :=
   | S0, S0 => True
   | _, _ => False
   end.
-  
+
 Definition one_thread_sampled_zero t1 t2 :=
   match t1, t2 with
   | S1 0, S0 => True
@@ -102,54 +78,30 @@ Definition one_thread_sampled_zero t1 t2 :=
 Definition at_least_one_thread_sampled_non_zero t1 t2 :=
   (match t1 with
    | S0 => False
-   | S1 n => n > 0 
+   | S1 n => n > 0
    | S2 n => n > 0
    end) ∨
   (match t2 with
    | S0 => False
-   | S1 n => n > 0 
+   | S1 n => n > 0
    | S2 n => n > 0
   end).
-    
-Canonical Structure TO := leibnizO T.
-
-Section lemmasT.
-  Context `{!inG Σ (excl_authR TO)}.
-
-  Lemma ghost_var_allocT b :
-    ⊢ |==> ∃ γ, own γ (●E b) ∗ own γ (◯E b).
-  Proof.
-    iMod (own_alloc (●E b ⋅ ◯E b)) as (γ) "[??]".
-    - by apply excl_auth_valid.
-    - by eauto with iFrame.
-  Qed.
-
-  Lemma ghost_var_agreeT γ b c :
-    own γ (●E b) -∗ own γ (◯E c) -∗ ⌜ b = c ⌝.
-  Proof.
-    iIntros "Hγ● Hγ◯".
-    by iCombine "Hγ● Hγ◯" gives %->%excl_auth_agree_L.
-  Qed.
-
-  Lemma ghost_var_updateT γ b' b c :
-    own γ (●E b) -∗ own γ (◯E c) ==∗ own γ (●E b') ∗ own γ (◯E b').
-  Proof.
-    iIntros "Hγ● Hγ◯".
-    iMod (own_update_2 _ _ _ (●E b' ⋅ ◯E b') with "Hγ● Hγ◯") as "[$$]".
-    { by apply excl_auth_update. }
-    done.
-  Qed.
-End lemmasT.
 
 Section complex'.
-  Context `{!conerisGS Σ, !spawnG Σ, !inG Σ (excl_authR TO)}.
+  Context `{!conerisGS Σ, !spawnG Σ, ghost_varG Σ T}.
+
+  (* The invariant needed for the parallel add.
+
+     The first line is ghost state omitted from the paper
+     discussion. See parallel_add_inv at the end of the file for an
+     alternate version that matches even more closely the syntactic
+     form of the paper *)
 
   Definition parallel_add_inv' (γ1 γ2: gname) l: iProp Σ :=
-    (* The first line is ghost state omitted from the paper discussion *)
-    ∃ (s1 s2 : T), own γ1 (●E s1) ∗ own γ2 (●E s2) ∗
+    ∃ (s1 s2 : T), ghost_var γ1 (1/2) s1 ∗ ghost_var γ2 (1/2) s2 ∗
       (((l ↦ #0 ∗ ⌜ no_thread_added s1 s2 ⌝) ∨
-         (∃ n : nat, l ↦ #n ∗ ⌜ one_thread_added s1 s2 n ⌝) ∨
-         (∃ n : nat, l ↦ #n ∗ ⌜ n > 0 ⌝ ∗ ⌜ both_threads_added s1 s2 n ⌝)) ∗
+         (∃ n : nat, l ↦ #n ∗ ⌜ one_thread_added n s1 s2 ⌝) ∨
+         (∃ n : nat, l ↦ #n ∗ ⌜ n > 0 ⌝ ∗ ⌜ both_threads_added n s1 s2 ⌝)) ∗
        ((↯(1/16) ∗ ⌜ no_thread_sampled s1 s2 ⌝) ∨
          (↯(1/4) ∗ ⌜ one_thread_sampled_zero s1 s2 ⌝) ∨
          (↯(1) (* both_thread_sampled_zero *)) ∨
@@ -164,14 +116,14 @@ Section complex'.
     iExists s2, s1.
     iFrame.
     iSplitL "Hstate".
-    { 
+    {
       iDestruct "Hstate" as "[H1|[H2|H3]]".
       { iLeft.  destruct s1, s2; naive_solver. }
       { iRight. iLeft. destruct s1, s2; naive_solver. }
       { iRight. iRight. rewrite /both_threads_added.
         iDestruct "H3" as "(%n&$&$&%Hp)"; iPureIntro; destruct s1, s2; try naive_solver; lia. }
     }
-    { 
+    {
       iDestruct "Hsamp" as "[H1|[H2|[H3|H4]]]".
       { iLeft.  destruct s1, s2; naive_solver. }
       { iRight. iLeft. destruct s1 as [|n1|n1]; destruct s2 as [|n2|n2]; try destruct n1, n2; naive_solver. }
@@ -184,15 +136,15 @@ Section complex'.
       }
     }
   Qed.
-  
+
   Lemma rand_step γ1 γ2 l:
-    {{{ inv nroot (parallel_add_inv' γ1 γ2 l) ∗ own γ1 (◯E S0) }}}
+    {{{ inv nroot (parallel_add_inv' γ1 γ2 l) ∗ ghost_var γ1 (1/2) S0 }}}
       rand #3
-      {{{ (n: nat), RET #n; own γ1 (◯E (S1 n)) }}}.
+      {{{ (n: nat), RET #n; ghost_var γ1 (1/2) (S1 n) }}}.
   Proof.
     iIntros (Φ) "(#I&Hfrag1) HΦ".
     iInv "I" as ">(%s1&%s2&Hauth1&Hauth2&Hstate&Hsamp)".
-    iDestruct (ghost_var_agreeT with "[$Hauth1][$]") as "->".
+    iDestruct (ghost_var_agree with "[$Hauth1][$]") as "->".
     iDestruct "Hsamp" as "[Hnosamp|[Hone0|[Hbogus|Honenonzero]]]".
     + iDestruct "Hnosamp" as "(Herr&%Hpure)".
       destruct s2; try inv Hpure; [].
@@ -202,10 +154,10 @@ Section complex'.
                         else 0)%R with "[$]") as (x) "Herr".
       { intros. case_match; last done. lra. }
       { rewrite SeriesC_finite_foldr. simpl. lra. }
-      iMod (ghost_var_updateT _ (S1 (fin_to_nat x)) with "[$Hauth1][$]") as "[Hauth1 Hfrag1]".
+      iMod (ghost_var_update_halves (S1 (fin_to_nat x)) with "[$Hauth1][$]") as "[Hauth1 Hfrag1]".
       iModIntro.
       iSplitL "Hauth1 Hauth2 Hstate Herr".
-      { iNext. iExists _, _.  iFrame "Hauth1 Hauth2 Hstate". 
+      { iNext. iExists _, _.  iFrame "Hauth1 Hauth2 Hstate".
         case_bool_decide as Hcase.
         * iRight. iLeft; iFrame. rewrite Hcase. by eauto.
         * iRight. iRight. iRight. iFrame. iPureIntro. rewrite /at_least_one_thread_sampled_non_zero. lia.
@@ -218,18 +170,18 @@ Section complex'.
                         else 0)%R with "[$]") as (x) "Herr".
       { intros. case_match; last done. lra. }
       { rewrite SeriesC_finite_foldr. simpl. lra. }
-      iMod (ghost_var_updateT _ (S1 (fin_to_nat x)) with "[$Hauth1][$]") as "[Hauth1 Hfrag1]".
+      iMod (ghost_var_update_halves (S1 (fin_to_nat x)) with "[$Hauth1][$]") as "[Hauth1 Hfrag1]".
       iModIntro.
       iSplitL "Hauth1 Hauth2 Hstate Herr".
-      { iNext. iExists _, _.  iFrame "Hauth1 Hauth2 Hstate". 
+      { iNext. iExists _, _.  iFrame "Hauth1 Hauth2 Hstate".
         case_bool_decide as Hcase.
-        * iFrame. 
+        * iFrame.
         * iRight. iRight. iRight. iFrame. iPureIntro. rewrite /at_least_one_thread_sampled_non_zero. lia.
       }
       by iApply "HΦ".
-    + iDestruct (ec_contradict with "Hbogus") as "[]". lra. 
+    + iDestruct (ec_contradict with "Hbogus") as "[]". lra.
     + wp_apply (wp_rand with "[//]") as (x) "_".
-      iMod (ghost_var_updateT _ (S1 (fin_to_nat x)) with "[$Hauth1][$]") as "[Hauth1 Hfrag1]".
+      iMod (ghost_var_update_halves (S1 (fin_to_nat x)) with "[$Hauth1][$]") as "[Hauth1 Hfrag1]".
       iModIntro.
       iSplitL "Hauth1 Hauth2 Hstate Honenonzero".
       { iNext. iExists _, _.  iFrame "Hauth1 Hauth2 Hstate".
@@ -240,20 +192,20 @@ Section complex'.
       }
       by iApply "HΦ".
   Qed.
-  
+
   Lemma faa_step γ1 γ2 l (n: nat) :
-    {{{ inv nroot (parallel_add_inv' γ1 γ2 l) ∗ own γ1 (◯E (S1 n)) }}}
+    {{{ inv nroot (parallel_add_inv' γ1 γ2 l) ∗ ghost_var γ1 (1/2) (S1 n) }}}
       FAA #l #n
-    {{{ (v : val), RET v; own γ1 (◯E (S2 n)) }}}.
+    {{{ (v : val), RET v; ghost_var γ1 (1/2) (S2 n) }}}.
   Proof.
     iIntros (Φ) "(#I&Hfrag1) HΦ".
     iInv "I" as ">(%s1&%s2&Hauth1&Hauth2&Hstate&Hsamp)".
-    iDestruct (ghost_var_agreeT with "[$Hauth1][$]") as "->".
+    iDestruct (ghost_var_agree with "[$Hauth1][$]") as "->".
     iDestruct "Hstate" as "[Hnone|[Hone|Htwo]]".
     * iDestruct "Hnone" as "(Hl&%Hcase)".
       wp_faa.
       iEval (simpl) in "Hl".
-      iMod (ghost_var_updateT _ (S2 n) with "[$Hauth1][$]") as "[Hauth1 Hfrag1]".
+      iMod (ghost_var_update_halves (S2 n) with "[$Hauth1][$]") as "[Hauth1 Hfrag1]".
       iModIntro.
       iSplitL "Hauth1 Hauth2 Hsamp Hl".
       { iNext. iExists _, _.  iFrame "Hauth1 Hauth2".
@@ -272,7 +224,7 @@ Section complex'.
     * iDestruct "Hone" as (n') "(Hl&%Hcase)".
       wp_faa.
       iEval (simpl) in "Hl".
-      iMod (ghost_var_updateT _ (S2 n) with "[$Hauth1][$]") as "[Hauth1 Hfrag1]".
+      iMod (ghost_var_update_halves (S2 n) with "[$Hauth1][$]") as "[Hauth1 Hfrag1]".
       destruct s2 as [| |n0]; try inversion Hcase.
       subst.
       iAssert (⌜at_least_one_thread_sampled_non_zero (S2 n) (S2 n0)⌝)%I as %Hatleast.
@@ -283,7 +235,7 @@ Section complex'.
         * eauto.
       }
       iMod (ec_zero) as "Hzero".
-      iMod (ghost_var_updateT _ (S2 n) with "[$Hauth1][$]") as "[Hauth1 Hfrag1]".
+      iMod (ghost_var_update_halves (S2 n) with "[$Hauth1][$]") as "[Hauth1 Hfrag1]".
       iModIntro.
       iSplitL "Hauth1 Hauth2 Hsamp Hl Hzero".
       { iNext. iExists _, _.  iFrame "Hauth1 Hauth2".
@@ -300,15 +252,15 @@ Section complex'.
     * iDestruct "Htwo" as (?) "(?&?&%Hp)".
       inversion Hp.
   Qed.
-  
+
   Lemma complex_parallel_add_spec':
     {{{ ↯ (1/16) }}}
       two_add_prog'
       {{{ (n:nat), RET #n; ⌜(0<n)%nat⌝ }}}.
   Proof.
     iIntros (Φ) "Herr HΦ".
-    iMod (ghost_var_allocT S0) as (γ1) "[Hauth1 Hfrag1]".
-    iMod (ghost_var_allocT S0) as (γ2) "[Hauth2 Hfrag2]".
+    iMod (ghost_var_alloc S0) as (γ1) "[Hauth1 Hfrag1]".
+    iMod (ghost_var_alloc S0) as (γ2) "[Hauth2 Hfrag2]".
     rewrite /two_add_prog'.
     wp_alloc l as "Hl".
     wp_pures.
@@ -320,9 +272,9 @@ Section complex'.
       { iPureIntro. left. by eauto. }
       { iLeft. iFrame. }
     }
-    wp_apply (wp_par (λ _, ∃ (n:nat), own γ1 (◯E (S2 n)))%I
-                (λ _, ∃ (n:nat), own γ2 (◯E (S2 n)))%I with "[Hfrag1][Hfrag2]").
-    - wp_apply (rand_step with "[$]"). 
+    wp_apply (wp_par (λ _, ∃ (n:nat), ghost_var γ1 (1/2) (S2 n))%I
+                (λ _, ∃ (n:nat), ghost_var γ2 (1/2) (S2 n))%I with "[Hfrag1][Hfrag2]").
+    - wp_apply (rand_step with "[$]").
       iIntros (n) "Hfrag1".
       wp_apply (faa_step with "[$]").
       iIntros (?) "Hfrag1".
@@ -332,7 +284,7 @@ Section complex'.
         iNext. iModIntro. iSplit; iIntros "H"; by iApply parallel_add_inv'_symmetric.
       }
       iClear "I".
-      wp_apply (rand_step with "[$]"). 
+      wp_apply (rand_step with "[$]").
       iIntros (n) "Hfrag1".
       wp_apply (faa_step with "[$]").
       iIntros (?) "Hfrag1".
@@ -340,8 +292,8 @@ Section complex'.
     - iIntros (??) "((%n1&H1)&(%n2&H2))".
       iNext. wp_pures.
       iInv "I" as ">(%s1&%s2&Hauth1&Hauth2&Hstate&Hsamp)".
-      iDestruct (ghost_var_agreeT with "[$Hauth1][$]") as "->".
-      iDestruct (ghost_var_agreeT with "[$Hauth2][$]") as "->".
+      iDestruct (ghost_var_agree with "[$Hauth1][$]") as "->".
+      iDestruct (ghost_var_agree with "[$Hauth2][$]") as "->".
       iDestruct "Hstate" as "[(?&%Hp)|[(%n&?&%Hp)|Htwo]]".
       { naive_solver. }
       { naive_solver. }
@@ -351,5 +303,74 @@ Section complex'.
       { iNext. iExists _, _; iFrame. iRight; iRight. iExists _; by iFrame. }
       iApply "HΦ". iPureIntro. lia.
   Qed.
-  
+
+  Definition gs γ1 γ2 P : iProp Σ :=
+    ∃ (s1 s2 : T), ghost_var γ1 (1/2/2) s1 ∗ ghost_var γ2 (1/2/2) s2 ∗ ⌜ P s1 s2 ⌝.
+
+  (* In the paper we do not have leading existentials in the descriptions of the invariant.
+     This alternate version matching the paper is defined next . It is equivalent to what
+     we used above. Essentially, in the paper each clause beginning with "gs γ1 γ2 [...]" is omitted *)
+
+  Definition parallel_add_inv (γ1 γ2: gname) l: iProp Σ :=
+      (((l ↦ #0 ∗ gs γ1 γ2 no_thread_added) ∨
+         (∃ n : nat, l ↦ #n ∗ gs γ1 γ2 (one_thread_added n)) ∨
+         (∃ n : nat, l ↦ #n ∗ ⌜ n > 0 ⌝ ∗ gs γ1 γ2 (both_threads_added n))) ∗
+       ((↯(1/16) ∗ gs γ1 γ2 no_thread_sampled) ∨
+         (↯(1/4) ∗ gs γ1 γ2 one_thread_sampled_zero) ∨
+         (↯(1) ∗ gs γ1 γ2 (λ _ _, True)) ∨
+         (↯(0) ∗ gs γ1 γ2 at_least_one_thread_sampled_non_zero))).
+
+  (* We now prove that the parallel_add_inv and parallel_add_inv' are equivalent *)
+
+  Lemma state_side_extract_gs γ1 γ2 l :
+   ((l ↦ #0 ∗ gs γ1 γ2 no_thread_added) ∨
+         (∃ n : nat, l ↦ #n ∗ gs γ1 γ2 (one_thread_added n)) ∨
+         (∃ n : nat, l ↦ #n ∗ ⌜ n > 0 ⌝ ∗ gs γ1 γ2 (both_threads_added n)))
+   -∗
+    ∃ (s1 s2 : T), ghost_var γ1 (1/2/2) s1 ∗ ghost_var γ2 (1/2/2) s2 ∗
+      (((l ↦ #0 ∗ ⌜ no_thread_added s1 s2 ⌝) ∨
+         (∃ n : nat, l ↦ #n ∗ ⌜ one_thread_added n s1 s2 ⌝) ∨
+         (∃ n : nat, l ↦ #n ∗ ⌜ n > 0 ⌝ ∗ ⌜ both_threads_added n s1 s2 ⌝))).
+  Proof.
+    iDestruct 1 as "[(?&(%s1&%s2&?&?&%Hp))|[(%n&Hl&%s1&%s2&?&?&%Hp)|(%n&Hl&%Hgt&%s1&%s2&?&?&%Hp)]]";
+      iExists s1, s2; iFrame; eauto with iFrame.
+  Qed.
+
+  Lemma samp_side_extract_gs γ1 γ2 :
+   ((↯(1/16) ∗ gs γ1 γ2 no_thread_sampled) ∨
+     (↯(1/4) ∗ gs γ1 γ2 one_thread_sampled_zero) ∨
+     (↯(1) ∗ gs γ1 γ2 (λ _ _, True : Prop)) ∨
+     (↯(0) ∗ gs γ1 γ2 at_least_one_thread_sampled_non_zero))
+   -∗
+    ∃ (s1 s2 : T), ghost_var γ1 (1/2/2) s1 ∗ ghost_var γ2 (1/2/2) s2 ∗
+       ((↯(1/16) ∗ ⌜ no_thread_sampled s1 s2 ⌝) ∨
+         (↯(1/4) ∗ ⌜ one_thread_sampled_zero s1 s2 ⌝) ∨
+         (↯(1) (* both_thread_sampled_zero *)) ∨
+         (↯(0) ∗ ⌜ at_least_one_thread_sampled_non_zero s1 s2 ⌝)).
+  Proof.
+    iIntros "H".
+    iDestruct "H" as "[H|[H|[H|H]]]";
+    iDestruct "H" as "(?&(%s1&%s2&?&?&%Hp))";
+      try iExists s1, s2; iFrame; eauto with iFrame.
+  Qed.
+
+  Lemma parallel_add_inv_equiv γ1 γ2 l :
+    parallel_add_inv γ1 γ2 l ∗-∗
+    parallel_add_inv' γ1 γ2 l.
+  Proof.
+    iSplit.
+    - iDestruct 1 as "(Hstate&Hsamp)".
+      iDestruct (state_side_extract_gs with "Hstate") as "(%s1&%s2&H1&H2&Hstate)".
+      iDestruct (samp_side_extract_gs with "Hsamp") as "(%s1'&%s2'&H1'&H2'&Hsamp)".
+      iDestruct (ghost_var_agree with "H1 H1'") as %<-.
+      iDestruct (ghost_var_agree with "H2 H2'") as %<-.
+      iExists s1, s2. iFrame.
+    - iDestruct 1 as "(%s1&%s2&Hauth1&Hauth2&Hstate&Hsamp)".
+      iDestruct "Hauth1" as "(Hauth1&Hauth1')".
+      iDestruct "Hauth2" as "(Hauth2&Hauth2')".
+      iSplitL "Hauth1 Hauth2 Hstate".
+      { iFrame. eauto. }
+      { iFrame. eauto. }
+  Qed.
+
 End complex'.
